format-version: 1.0
data-version: 1
date: 05:24:2016 03:00
saved-by: cass
default-namespace: cass_tissue_ontology
remark: none
ontology: cass_tissue

[Term]
id: CASSTISS:0000000
name: cass_tissues

[Term]
id: CASSTISS:0000001
name: cass leaf
synonym: "Lf" EXACT
def: "" []
is_a: CASSTISS:0000000

[Term]
id: CASSTISS:0000002
name: cass stem
synonym: "Stm" EXACT
def: "" []
is_a: CASSTISS:0000000

[Term]
id: CASSTISS:0000003
name: cass root
synonym: "Rt" EXACT
def: "" []
is_a: CASSTISS:0000000

[Term]
id: CASSTISS:0000004
name: cass sink leaf
synonym: "SnkLf" EXACT
def: "" []
is_a: CASSTISS:0000001

[Term]
id: CASSTISS:0000005
name: cass source leaf
synonym: "SrcLf" EXACT
def: "" []
is_a: CASSTISS:0000001

[Term]
id: CASSTISS:0000006
name: cass lower leaf
synonym: "LwrLf" EXACT
def: "" []
is_a: CASSTISS:0000001

[Term]
id: CASSTISS:0000007
name: cass upper stem
synonym: "UpStm" EXACT
def: "Green and not woody." []
is_a: CASSTISS:0000002

[Term]
id: CASSTISS:0000008
name: cass lower stem
synonym: "LwrStm" EXACT
def: "" []
is_a: CASSTISS:0000002

[Term]
id: CASSTISS:0000009
name: cass lower stem whole
synonym: "LwrStmWhl" EXACT
def: "" []
is_a: CASSTISS:0000008

[Term]
id: CASSTISS:0000010
name: cass lower stem bark
synonym: "LwStmBrk" EXACT
def: "" []
is_a: CASSTISS:0000008

[Term]
id: CASSTISS:0000011
name: cass fibrous root
synonym: "FbrRt" EXACT
def: "" []
is_a: CASSTISS:0000003

[Term]
id: CASSTISS:0000012
name: cass pre-storage root
synonym: "PreStrRt" EXACT
def: "Potential storage root." []
is_a: CASSTISS:0000003

[Term]
id: CASSTISS:0000013
name: cass storage root
synonym: "StrRt" EXACT
def: "" []
is_a: CASSTISS:0000003

[Term]
id: CASSTISS:0000014
name: mother plant stem
def: "The position of the stem on the mother plant from which this plant was replanted. 1 is the lowest position." []
is_a: CASSTISS:0000000

[Term]
id: CASSTISS:0000015
name: stick 1
def: "The position of the stem on the mother plant from which this plant was replanted. 1 is the lowest position, which is this term." []
is_a: CASSTISS:0000014

[Term]
id: CASSTISS:0000016
name: stick 2
def: "The position of the stem on the mother plant from which this plant was replanted. 1 is the lowest position. This term is position 2." []
is_a: CASSTISS:0000014

[Term]
id: CASSTISS:0000017
name: stick 3
def: "The position of the stem on the mother plant from which this plant was replanted. 1 is the lowest position. This term is position 3." []
is_a: CASSTISS:0000014
