format-version: 1.0
data-version: 1
date: 05:23:2016 03:00
saved-by: cass
default-namespace: cass_time_ontology
remark: none
ontology: cass_time

[Term]
id: CASSTIME:0000000
name: cass_time_terms

[Term]
id: CASSTIME:0000001
name: cass time of day
def: "Categorical day periods." []
is_a: CASSTIME:0000000

[Term]
id: CASSTIME:0000002
name: cass end of night
synonym: "EoN" EXACT
def: "Half an hour before sunrise." []
is_a: CASSTIME:0000001

[Term]
id: CASSTIME:0000003
name: cass end of day
synonym: "EoD" EXACT
def: "Late afternoon daylight." []
is_a: CASSTIME:0000001

[Term]
id: CASSTIME:0000004
name: cass mid day
synonym: "MD" EXACT
def: "Between 11:00 in the morning and 14:00 in the afternoon." []
is_a: CASSTIME:0000001

[Term]
id: CASSTIME:0000005
name: cass number of weeks
def: "Number of weeks." []
is_a: CASSTIME:0000000

[Term]
id: CASSTIME:0000006
name: cass week 1
synonym: "Wk1" EXACT
def: "" []
is_a: CASSTIME:0000005

[Term]
id: CASSTIME:0000007
name: cass week 2
synonym: "Wk2" EXACT
def: "" []
is_a: CASSTIME:0000005

[Term]
id: CASSTIME:0000008
name: cass week 3
synonym: "Wk3" EXACT
def: "" []
is_a: CASSTIME:0000005

[Term]
id: CASSTIME:0000009
name: cass week 4
synonym: "Wk4" EXACT
def: "" []
is_a: CASSTIME:0000005

[Term]
id: CASSTIME:0000010
name: cass week 5
synonym: "Wk5" EXACT
def: "" []
is_a: CASSTIME:0000005

[Term]
id: CASSTIME:0000011
name: cass week 6
synonym: "Wk6" EXACT
def: "" []
is_a: CASSTIME:0000005

[Term]
id: CASSTIME:0000012
name: cass week 7
synonym: "Wk7" EXACT
def: "" []
is_a: CASSTIME:0000005

[Term]
id: CASSTIME:0000013
name: cass week 8
synonym: "Wk8" EXACT
def: "" []
is_a: CASSTIME:0000005

[Term]
id: CASSTIME:0000014
name: cass week 9
synonym: "Wk9" EXACT
def: "" []
is_a: CASSTIME:0000005

[Term]
id: CASSTIME:0000015
name: cass week 10
synonym: "Wk10" EXACT
def: "" []
is_a: CASSTIME:0000005

[Term]
id: CASSTIME:0000016
name: cass week 11
synonym: "Wk11" EXACT
def: "" []
is_a: CASSTIME:0000005

[Term]
id: CASSTIME:0000017
name: cass week 12
synonym: "Wk12" EXACT
def: "" []
is_a: CASSTIME:0000005

[Term]
id: CASSTIME:0000018
name: cass week 13
synonym: "Wk13" EXACT
def: "" []
is_a: CASSTIME:0000005

[Term]
id: CASSTIME:0000019
name: cass week 14
synonym: "Wk14" EXACT
def: "" []
is_a: CASSTIME:0000005

[Term]
id: CASSTIME:0000020
name: cass week 15
synonym: "Wk15" EXACT
def: "" []
is_a: CASSTIME:0000005

[Term]
id: CASSTIME:0000021
name: cass week 16
synonym: "Wk16" EXACT
def: "" []
is_a: CASSTIME:0000005

[Term]
id: CASSTIME:0000022
name: cass week 17
synonym: "Wk17" EXACT
def: "" []
is_a: CASSTIME:0000005

[Term]
id: CASSTIME:0000023
name: cass week 18
synonym: "Wk18" EXACT
def: "" []
is_a: CASSTIME:0000005

[Term]
id: CASSTIME:0000024
name: cass week 19
synonym: "Wk19" EXACT
def: "" []
is_a: CASSTIME:0000005

[Term]
id: CASSTIME:0000025
name: cass week 20
synonym: "Wk20" EXACT
def: "" []
is_a: CASSTIME:0000005

[Term]
id: CASSTIME:0000026
name: cass week 21
synonym: "Wk21" EXACT
def: "" []
is_a: CASSTIME:0000005

[Term]
id: CASSTIME:0000027
name: cass week 22
synonym: "Wk22" EXACT
def: "" []
is_a: CASSTIME:0000005

[Term]
id: CASSTIME:0000028
name: cass week 23
synonym: "Wk23" EXACT
def: "" []
is_a: CASSTIME:0000005

[Term]
id: CASSTIME:0000029
name: cass week 24
synonym: "Wk24" EXACT
def: "" []
is_a: CASSTIME:0000005

[Term]
id: CASSTIME:0000030
name: cass week 25
synonym: "Wk25" EXACT
def: "" []
is_a: CASSTIME:0000005

[Term]
id: CASSTIME:0000031
name: cass week 26
synonym: "Wk26" EXACT
def: "" []
is_a: CASSTIME:0000005

[Term]
id: CASSTIME:0000032
name: cass week 27
synonym: "Wk27" EXACT
def: "" []
is_a: CASSTIME:0000005

[Term]
id: CASSTIME:0000033
name: cass week 28
synonym: "Wk28" EXACT
def: "" []
is_a: CASSTIME:0000005

[Term]
id: CASSTIME:0000034
name: cass week 29
synonym: "Wk29" EXACT
def: "" []
is_a: CASSTIME:0000005

[Term]
id: CASSTIME:0000035
name: cass week 30
synonym: "Wk30" EXACT
def: "" []
is_a: CASSTIME:0000005

[Term]
id: CASSTIME:0000036
name: cass week 31
synonym: "Wk31" EXACT
def: "" []
is_a: CASSTIME:0000005

[Term]
id: CASSTIME:0000037
name: cass week 32
synonym: "Wk32" EXACT
def: "" []
is_a: CASSTIME:0000005

[Term]
id: CASSTIME:0000038
name: cass week 33
synonym: "Wk33" EXACT
def: "" []
is_a: CASSTIME:0000005

[Term]
id: CASSTIME:0000039
name: cass week 34
synonym: "Wk34" EXACT
def: "" []
is_a: CASSTIME:0000005

[Term]
id: CASSTIME:0000040
name: cass week 35
synonym: "Wk35" EXACT
def: "" []
is_a: CASSTIME:0000005

[Term]
id: CASSTIME:0000041
name: cass week 36
synonym: "Wk36" EXACT
def: "" []
is_a: CASSTIME:0000005

[Term]
id: CASSTIME:0000042
name: cass week 37
synonym: "Wk37" EXACT
def: "" []
is_a: CASSTIME:0000005

[Term]
id: CASSTIME:0000043
name: cass week 38
synonym: "Wk38" EXACT
def: "" []
is_a: CASSTIME:0000005

[Term]
id: CASSTIME:0000044
name: cass week 39
synonym: "Wk39" EXACT
def: "" []
is_a: CASSTIME:0000005

[Term]
id: CASSTIME:0000045
name: cass week 40
synonym: "Wk40" EXACT
def: "" []
is_a: CASSTIME:0000005

[Term]
id: CASSTIME:0000046
name: cass week 41
synonym: "Wk41" EXACT
def: "" []
is_a: CASSTIME:0000005

[Term]
id: CASSTIME:0000047
name: cass week 42
synonym: "Wk42" EXACT
def: "" []
is_a: CASSTIME:0000005

[Term]
id: CASSTIME:0000048
name: cass week 43
synonym: "Wk43" EXACT
def: "" []
is_a: CASSTIME:0000005

[Term]
id: CASSTIME:0000049
name: cass week 44
synonym: "Wk44" EXACT
def: "" []
is_a: CASSTIME:0000005

[Term]
id: CASSTIME:0000050
name: cass week 45
synonym: "Wk45" EXACT
def: "" []
is_a: CASSTIME:0000005

[Term]
id: CASSTIME:0000051
name: cass week 46
synonym: "Wk46" EXACT
def: "" []
is_a: CASSTIME:0000005

[Term]
id: CASSTIME:0000052
name: cass week 47
synonym: "Wk47" EXACT
def: "" []
is_a: CASSTIME:0000005

[Term]
id: CASSTIME:0000053
name: cass week 48
synonym: "Wk48" EXACT
def: "" []
is_a: CASSTIME:0000005

[Term]
id: CASSTIME:0000054
name: cass week 49
synonym: "Wk49" EXACT
def: "" []
is_a: CASSTIME:0000005

[Term]
id: CASSTIME:0000055
name: cass week 50
synonym: "Wk50" EXACT
def: "" []
is_a: CASSTIME:0000005

[Term]
id: CASSTIME:0000056
name: cass week 51
synonym: "Wk51" EXACT
def: "" []
is_a: CASSTIME:0000005

[Term]
id: CASSTIME:0000057
name: cass week 52
synonym: "Wk52" EXACT
def: "" []
is_a: CASSTIME:0000005

[Term]
id: CASSTIME:0000058
name: cass week 53
synonym: "Wk53" EXACT
def: "" []
is_a: CASSTIME:0000005

[Term]
id: CASSTIME:0000059
name: cass week 54
synonym: "Wk54" EXACT
def: "" []
is_a: CASSTIME:0000005

[Term]
id: CASSTIME:0000134
name: cass week 55
synonym: "Wk55" EXACT
def: "" []
is_a: CASSTIME:0000005

[Term]
id: CASSTIME:0000135
name: cass week 56
synonym: "Wk56" EXACT
def: "" []
is_a: CASSTIME:0000005

[Term]
id: CASSTIME:0000136
name: cass week 57
synonym: "Wk57" EXACT
def: "" []
is_a: CASSTIME:0000005

[Term]
id: CASSTIME:0000137
name: cass week 58
synonym: "Wk58" EXACT
def: "" []
is_a: CASSTIME:0000005

[Term]
id: CASSTIME:0000138
name: cass week 59
synonym: "Wk59" EXACT
def: "" []
is_a: CASSTIME:0000005

[Term]
id: CASSTIME:0000139
name: cass week 60
synonym: "Wk60" EXACT
def: "" []
is_a: CASSTIME:0000005

[Term]
id: CASSTIME:0000140
name: cass week 61
synonym: "Wk61" EXACT
def: "" []
is_a: CASSTIME:0000005

[Term]
id: CASSTIME:0000141
name: cass week 62
synonym: "Wk62" EXACT
def: "" []
is_a: CASSTIME:0000005

[Term]
id: CASSTIME:0000142
name: cass week 63
synonym: "Wk63" EXACT
def: "" []
is_a: CASSTIME:0000005

[Term]
id: CASSTIME:0000143
name: cass week 64
synonym: "Wk64" EXACT
def: "" []
is_a: CASSTIME:0000005

[Term]
id: CASSTIME:0000144
name: cass week 65
synonym: "Wk65" EXACT
def: "" []
is_a: CASSTIME:0000005

[Term]
id: CASSTIME:0000145
name: cass week 66
synonym: "Wk66" EXACT
def: "" []
is_a: CASSTIME:0000005

[Term]
id: CASSTIME:0000146
name: cass week 67
synonym: "Wk67" EXACT
def: "" []
is_a: CASSTIME:0000005

[Term]
id: CASSTIME:0000147
name: cass week 68
synonym: "Wk68" EXACT
def: "" []
is_a: CASSTIME:0000005

[Term]
id: CASSTIME:0000148
name: cass week 69
synonym: "Wk69" EXACT
def: "" []
is_a: CASSTIME:0000005

[Term]
id: CASSTIME:0000149
name: cass week 70
synonym: "Wk70" EXACT
def: "" []
is_a: CASSTIME:0000005

[Term]
id: CASSTIME:0000150
name: cass week 71
synonym: "Wk71" EXACT
def: "" []
is_a: CASSTIME:0000005

[Term]
id: CASSTIME:0000151
name: cass week 72
synonym: "Wk72" EXACT
def: "" []
is_a: CASSTIME:0000005

[Term]
id: CASSTIME:0000152
name: cass week 73
synonym: "Wk73" EXACT
def: "" []
is_a: CASSTIME:0000005

[Term]
id: CASSTIME:0000153
name: cass week 74
synonym: "Wk74" EXACT
def: "" []
is_a: CASSTIME:0000005

[Term]
id: CASSTIME:0000154
name: cass week 75
synonym: "Wk75" EXACT
def: "" []
is_a: CASSTIME:0000005

[Term]
id: CASSTIME:0000155
name: cass week 76
synonym: "Wk76" EXACT
def: "" []
is_a: CASSTIME:0000005

[Term]
id: CASSTIME:0000156
name: cass week 77
synonym: "Wk77" EXACT
def: "" []
is_a: CASSTIME:0000005

[Term]
id: CASSTIME:0000157
name: cass week 78
synonym: "Wk78" EXACT
def: "" []
is_a: CASSTIME:0000005

[Term]
id: CASSTIME:0000158
name: cass week 79
synonym: "Wk79" EXACT
def: "" []
is_a: CASSTIME:0000005

[Term]
id: CASSTIME:0000159
name: cass week 80
synonym: "Wk80" EXACT
def: "" []
is_a: CASSTIME:0000005

[Term]
id: CASSTIME:0000060
name: cass months
def: "Months." []
is_a: CASSTIME:0000000

[Term]
id: CASSTIME:0000061
name: cass month 1
synonym: "Mo1" EXACT
def: "" []
is_a: CASSTIME:0000060

[Term]
id: CASSTIME:0000061
name: cass month 1
synonym: "Mo1" EXACT
def: "" []
is_a: CASSTIME:0000060

[Term]
id: CASSTIME:0000061
name: cass month 1
synonym: "Mo1" EXACT
def: "" []
is_a: CASSTIME:0000060

[Term]
id: CASSTIME:0000061
name: cass month 1
synonym: "Mo1" EXACT
def: "" []
is_a: CASSTIME:0000060

[Term]
id: CASSTIME:0000062
name: cass month 2
synonym: "Mo2" EXACT
def: "" []
is_a: CASSTIME:0000060

[Term]
id: CASSTIME:0000063
name: cass month 3
synonym: "Mo3" EXACT
def: "" []
is_a: CASSTIME:0000060

[Term]
id: CASSTIME:0000064
name: cass month 4
synonym: "Mo4" EXACT
def: "" []
is_a: CASSTIME:0000060

[Term]
id: CASSTIME:0000065
name: cass month 5
synonym: "Mo5" EXACT
def: "" []
is_a: CASSTIME:0000060

[Term]
id: CASSTIME:0000066
name: cass month 6
synonym: "Mo6" EXACT
def: "" []
is_a: CASSTIME:0000060

[Term]
id: CASSTIME:0000067
name: cass month 7
synonym: "Mo7" EXACT
def: "" []
is_a: CASSTIME:0000060

[Term]
id: CASSTIME:0000068
name: cass month 8
synonym: "Mo8" EXACT
def: "" []
is_a: CASSTIME:0000060

[Term]
id: CASSTIME:0000069
name: cass month 9
synonym: "Mo9" EXACT
def: "" []
is_a: CASSTIME:0000060

[Term]
id: CASSTIME:0000070
name: cass month 10
synonym: "Mo10" EXACT
def: "" []
is_a: CASSTIME:0000060

[Term]
id: CASSTIME:0000071
name: cass month 11
synonym: "Mo11" EXACT
def: "" []
is_a: CASSTIME:0000060

[Term]
id: CASSTIME:0000072
name: cass month 12
synonym: "Mo12" EXACT
def: "" []
is_a: CASSTIME:0000060

[Term]
id: CASSTIME:0000073
name: cass number of days
def: "Number of days." []
is_a: CASSTIME:0000000

[Term]
id: CASSTIME:0000074
name: cass day 1
synonym: "day1" EXACT
def: "" []
is_a: CASSTIME:0000073

[Term]
id: CASSTIME:0000075
name: cass day 2
synonym: "day2" EXACT
def: "" []
is_a: CASSTIME:0000073

[Term]
id: CASSTIME:0000076
name: cass day 3
synonym: "day3" EXACT
def: "" []
is_a: CASSTIME:0000073

[Term]
id: CASSTIME:0000077
name: cass day 4
synonym: "day4" EXACT
def: "" []
is_a: CASSTIME:0000073

[Term]
id: CASSTIME:0000078
name: cass day 5
synonym: "day5" EXACT
def: "" []
is_a: CASSTIME:0000073

[Term]
id: CASSTIME:0000079
name: cass day 6
synonym: "day6" EXACT
def: "" []
is_a: CASSTIME:0000073

[Term]
id: CASSTIME:0000080
name: cass day 7
synonym: "day7" EXACT
def: "" []
is_a: CASSTIME:0000073

[Term]
id: CASSTIME:0000081
name: cass day 8
synonym: "day8" EXACT
def: "" []
is_a: CASSTIME:0000073

[Term]
id: CASSTIME:0000082
name: cass day 9
synonym: "day9" EXACT
def: "" []
is_a: CASSTIME:0000073

[Term]
id: CASSTIME:0000083
name: cass day 10
synonym: "day10" EXACT
def: "" []
is_a: CASSTIME:0000073

[Term]
id: CASSTIME:0000084
name: cass day 11
synonym: "day11" EXACT
def: "" []
is_a: CASSTIME:0000073

[Term]
id: CASSTIME:0000085
name: cass day 12
synonym: "day12" EXACT
def: "" []
is_a: CASSTIME:0000073

[Term]
id: CASSTIME:0000086
name: cass day 13
synonym: "day13" EXACT
def: "" []
is_a: CASSTIME:0000073

[Term]
id: CASSTIME:0000087
name: cass day 14
synonym: "day14" EXACT
def: "" []
is_a: CASSTIME:0000073

[Term]
id: CASSTIME:0000088
name: cass day 15
synonym: "day15" EXACT
def: "" []
is_a: CASSTIME:0000073

[Term]
id: CASSTIME:0000089
name: cass day 16
synonym: "day16" EXACT
def: "" []
is_a: CASSTIME:0000073

[Term]
id: CASSTIME:0000090
name: cass day 17
synonym: "day17" EXACT
def: "" []
is_a: CASSTIME:0000073

[Term]
id: CASSTIME:0000091
name: cass day 18
synonym: "day18" EXACT
def: "" []
is_a: CASSTIME:0000073

[Term]
id: CASSTIME:0000092
name: cass day 19
synonym: "day19" EXACT
def: "" []
is_a: CASSTIME:0000073

[Term]
id: CASSTIME:0000093
name: cass day 20
synonym: "day20" EXACT
def: "" []
is_a: CASSTIME:0000073

[Term]
id: CASSTIME:0000094
name: cass day 21
synonym: "day21" EXACT
def: "" []
is_a: CASSTIME:0000073

[Term]
id: CASSTIME:0000095
name: cass day 22
synonym: "day22" EXACT
def: "" []
is_a: CASSTIME:0000073

[Term]
id: CASSTIME:0000096
name: cass day 23
synonym: "day23" EXACT
def: "" []
is_a: CASSTIME:0000073

[Term]
id: CASSTIME:0000097
name: cass day 24
synonym: "day24" EXACT
def: "" []
is_a: CASSTIME:0000073

[Term]
id: CASSTIME:0000098
name: cass day 25
synonym: "day25" EXACT
def: "" []
is_a: CASSTIME:0000073

[Term]
id: CASSTIME:0000099
name: cass day 26
synonym: "day26" EXACT
def: "" []
is_a: CASSTIME:0000073

[Term]
id: CASSTIME:0000100
name: cass day 27
synonym: "day27" EXACT
def: "" []
is_a: CASSTIME:0000073

[Term]
id: CASSTIME:0000101
name: cass day 28
synonym: "day28" EXACT
def: "" []
is_a: CASSTIME:0000073

[Term]
id: CASSTIME:0000102
name: cass day 29
synonym: "day29" EXACT
def: "" []
is_a: CASSTIME:0000073

[Term]
id: CASSTIME:0000103
name: cass day 30
synonym: "day30" EXACT
def: "" []
is_a: CASSTIME:0000073

[Term]
id: CASSTIME:0000104
name: cass day 31
synonym: "day31" EXACT
def: "" []
is_a: CASSTIME:0000073

[Term]
id: CASSTIME:0000105
name: cass day 32
synonym: "day32" EXACT
def: "" []
is_a: CASSTIME:0000073

[Term]
id: CASSTIME:0000106
name: cass day 33
synonym: "day33" EXACT
def: "" []
is_a: CASSTIME:0000073

[Term]
id: CASSTIME:0000107
name: cass day 34
synonym: "day34" EXACT
def: "" []
is_a: CASSTIME:0000073

[Term]
id: CASSTIME:0000108
name: cass day 35
synonym: "day35" EXACT
def: "" []
is_a: CASSTIME:0000073

[Term]
id: CASSTIME:0000109
name: cass day 36
synonym: "day36" EXACT
def: "" []
is_a: CASSTIME:0000073

[Term]
id: CASSTIME:0000110
name: cass day 37
synonym: "day37" EXACT
def: "" []
is_a: CASSTIME:0000073

[Term]
id: CASSTIME:0000111
name: cass day 38
synonym: "day38" EXACT
def: "" []
is_a: CASSTIME:0000073

[Term]
id: CASSTIME:0000112
name: cass day 39
synonym: "day39" EXACT
def: "" []
is_a: CASSTIME:0000073

[Term]
id: CASSTIME:0000113
name: cass day 40
synonym: "day40" EXACT
def: "" []
is_a: CASSTIME:0000073

[Term]
id: CASSTIME:0000114
name: cass day 41
synonym: "day41" EXACT
def: "" []
is_a: CASSTIME:0000073

[Term]
id: CASSTIME:0000115
name: cass day 42
synonym: "day42" EXACT
def: "" []
is_a: CASSTIME:0000073

[Term]
id: CASSTIME:0000116
name: cass day 43
synonym: "day43" EXACT
def: "" []
is_a: CASSTIME:0000073

[Term]
id: CASSTIME:0000117
name: cass day 44
synonym: "day44" EXACT
def: "" []
is_a: CASSTIME:0000073

[Term]
id: CASSTIME:0000118
name: cass day 45
synonym: "day45" EXACT
def: "" []
is_a: CASSTIME:0000073

[Term]
id: CASSTIME:0000119
name: cass day 46
synonym: "day46" EXACT
def: "" []
is_a: CASSTIME:0000073

[Term]
id: CASSTIME:0000120
name: cass day 47
synonym: "day47" EXACT
def: "" []
is_a: CASSTIME:0000073

[Term]
id: CASSTIME:0000121
name: cass day 48
synonym: "day48" EXACT
def: "" []
is_a: CASSTIME:0000073

[Term]
id: CASSTIME:0000122
name: cass day 49
synonym: "day49" EXACT
def: "" []
is_a: CASSTIME:0000073

[Term]
id: CASSTIME:0000123
name: cass day 50
synonym: "day50" EXACT
def: "" []
is_a: CASSTIME:0000073

[Term]
id: CASSTIME:0000124
name: cass day 51
synonym: "day51" EXACT
def: "" []
is_a: CASSTIME:0000073

[Term]
id: CASSTIME:0000125
name: cass day 52
synonym: "day52" EXACT
def: "" []
is_a: CASSTIME:0000073

[Term]
id: CASSTIME:0000126
name: cass day 53
synonym: "day53" EXACT
def: "" []
is_a: CASSTIME:0000073

[Term]
id: CASSTIME:0000127
name: cass day 54
synonym: "day54" EXACT
def: "" []
is_a: CASSTIME:0000073

[Term]
id: CASSTIME:0000128
name: cass day 55
synonym: "day55" EXACT
def: "" []
is_a: CASSTIME:0000073

[Term]
id: CASSTIME:0000129
name: cass day 56
synonym: "day56" EXACT
def: "" []
is_a: CASSTIME:0000073

[Term]
id: CASSTIME:0000130
name: cass day 57
synonym: "day57" EXACT
def: "" []
is_a: CASSTIME:0000073

[Term]
id: CASSTIME:0000131
name: cass day 58
synonym: "day58" EXACT
def: "" []
is_a: CASSTIME:0000073

[Term]
id: CASSTIME:0000132
name: cass day 59
synonym: "day59" EXACT
def: "" []
is_a: CASSTIME:0000073

[Term]
id: CASSTIME:0000133
name: cass day 60
synonym: "day60" EXACT
def: "" []
is_a: CASSTIME:0000073

[Term]
id: CASSTIME:0000134
name: cass day 61
synonym: "day61" EXACT
def: "" []
is_a: CASSTIME:0000073

[Term]
id: CASSTIME:0000135
name: cass day 62
synonym: "day62" EXACT
def: "" []
is_a: CASSTIME:0000073

[Term]
id: CASSTIME:0000136
name: cass day 63
synonym: "day63" EXACT
def: "" []
is_a: CASSTIME:0000073

[Term]
id: CASSTIME:0000137
name: cass day 64
synonym: "day64" EXACT
def: "" []
is_a: CASSTIME:0000073

[Term]
id: CASSTIME:0000138
name: cass day 65
synonym: "day65" EXACT
def: "" []
is_a: CASSTIME:0000073

[Term]
id: CASSTIME:0000139
name: cass day 66
synonym: "day66" EXACT
def: "" []
is_a: CASSTIME:0000073

[Term]
id: CASSTIME:0000140
name: cass day 67
synonym: "day67" EXACT
def: "" []
is_a: CASSTIME:0000073

[Term]
id: CASSTIME:0000141
name: cass day 68
synonym: "day68" EXACT
def: "" []
is_a: CASSTIME:0000073

[Term]
id: CASSTIME:0000142
name: cass day 69
synonym: "day69" EXACT
def: "" []
is_a: CASSTIME:0000073

[Term]
id: CASSTIME:0000143
name: cass day 70
synonym: "day70" EXACT
def: "" []
is_a: CASSTIME:0000073

[Term]
id: CASSTIME:0000144
name: cass day 71
synonym: "day71" EXACT
def: "" []
is_a: CASSTIME:0000073

[Term]
id: CASSTIME:0000145
name: cass day 72
synonym: "day72" EXACT
def: "" []
is_a: CASSTIME:0000073

[Term]
id: CASSTIME:0000146
name: cass day 73
synonym: "day73" EXACT
def: "" []
is_a: CASSTIME:0000073

[Term]
id: CASSTIME:0000147
name: cass day 74
synonym: "day74" EXACT
def: "" []
is_a: CASSTIME:0000073

[Term]
id: CASSTIME:0000148
name: cass day 75
synonym: "day75" EXACT
def: "" []
is_a: CASSTIME:0000073

[Term]
id: CASSTIME:0000149
name: cass day 76
synonym: "day76" EXACT
def: "" []
is_a: CASSTIME:0000073

[Term]
id: CASSTIME:0000150
name: cass day 77
synonym: "day77" EXACT
def: "" []
is_a: CASSTIME:0000073

[Term]
id: CASSTIME:0000151
name: cass day 78
synonym: "day78" EXACT
def: "" []
is_a: CASSTIME:0000073

[Term]
id: CASSTIME:0000152
name: cass day 79
synonym: "day79" EXACT
def: "" []
is_a: CASSTIME:0000073

[Term]
id: CASSTIME:0000153
name: cass day 80
synonym: "day80" EXACT
def: "" []
is_a: CASSTIME:0000073

[Term]
id: CASSTIME:0000154
name: cass day 81
synonym: "day81" EXACT
def: "" []
is_a: CASSTIME:0000073

[Term]
id: CASSTIME:0000155
name: cass day 82
synonym: "day82" EXACT
def: "" []
is_a: CASSTIME:0000073

[Term]
id: CASSTIME:0000156
name: cass day 83
synonym: "day83" EXACT
def: "" []
is_a: CASSTIME:0000073

[Term]
id: CASSTIME:0000157
name: cass day 84
synonym: "day84" EXACT
def: "" []
is_a: CASSTIME:0000073

[Term]
id: CASSTIME:0000158
name: cass day 85
synonym: "day85" EXACT
def: "" []
is_a: CASSTIME:0000073

[Term]
id: CASSTIME:0000159
name: cass day 86
synonym: "day86" EXACT
def: "" []
is_a: CASSTIME:0000073

[Term]
id: CASSTIME:0000160
name: cass day 87
synonym: "day87" EXACT
def: "" []
is_a: CASSTIME:0000073

[Term]
id: CASSTIME:0000161
name: cass day 88
synonym: "day88" EXACT
def: "" []
is_a: CASSTIME:0000073

[Term]
id: CASSTIME:0000162
name: cass day 89
synonym: "day89" EXACT
def: "" []
is_a: CASSTIME:0000073

[Term]
id: CASSTIME:0000163
name: cass day 90
synonym: "day90" EXACT
def: "" []
is_a: CASSTIME:0000073

[Term]
id: CASSTIME:0000164
name: cass day 91
synonym: "day91" EXACT
def: "" []
is_a: CASSTIME:0000073

[Term]
id: CASSTIME:0000165
name: cass day 92
synonym: "day92" EXACT
def: "" []
is_a: CASSTIME:0000073

[Term]
id: CASSTIME:0000166
name: cass day 93
synonym: "day93" EXACT
def: "" []
is_a: CASSTIME:0000073

[Term]
id: CASSTIME:0000167
name: cass day 94
synonym: "day94" EXACT
def: "" []
is_a: CASSTIME:0000073

[Term]
id: CASSTIME:0000168
name: cass day 95
synonym: "day95" EXACT
def: "" []
is_a: CASSTIME:0000073

[Term]
id: CASSTIME:0000169
name: cass day 96
synonym: "day96" EXACT
def: "" []
is_a: CASSTIME:0000073

[Term]
id: CASSTIME:0000170
name: cass day 97
synonym: "day97" EXACT
def: "" []
is_a: CASSTIME:0000073

[Term]
id: CASSTIME:0000171
name: cass day 98
synonym: "day98" EXACT
def: "" []
is_a: CASSTIME:0000073

[Term]
id: CASSTIME:0000172
name: cass day 99
synonym: "day99" EXACT
def: "" []
is_a: CASSTIME:0000073

[Term]
id: CASSTIME:0000173
name: cass day 100
synonym: "day100" EXACT
def: "" []
is_a: CASSTIME:0000073

[Term]
id: CASSTIME:0000174
name: cass day 101
synonym: "day101" EXACT
def: "" []
is_a: CASSTIME:0000073

[Term]
id: CASSTIME:0000175
name: cass day 102
synonym: "day102" EXACT
def: "" []
is_a: CASSTIME:0000073

[Term]
id: CASSTIME:0000176
name: cass day 103
synonym: "day103" EXACT
def: "" []
is_a: CASSTIME:0000073

[Term]
id: CASSTIME:0000177
name: cass day 104
synonym: "day104" EXACT
def: "" []
is_a: CASSTIME:0000073

[Term]
id: CASSTIME:0000178
name: cass day 105
synonym: "day105" EXACT
def: "" []
is_a: CASSTIME:0000073

[Term]
id: CASSTIME:0000179
name: cass day 106
synonym: "day106" EXACT
def: "" []
is_a: CASSTIME:0000073

[Term]
id: CASSTIME:0000180
name: cass day 107
synonym: "day107" EXACT
def: "" []
is_a: CASSTIME:0000073

[Term]
id: CASSTIME:0000181
name: cass day 108
synonym: "day108" EXACT
def: "" []
is_a: CASSTIME:0000073

[Term]
id: CASSTIME:0000182
name: cass day 109
synonym: "day109" EXACT
def: "" []
is_a: CASSTIME:0000073

[Term]
id: CASSTIME:0000183
name: cass day 110
synonym: "day110" EXACT
def: "" []
is_a: CASSTIME:0000073

[Term]
id: CASSTIME:0000184
name: cass day 111
synonym: "day111" EXACT
def: "" []
is_a: CASSTIME:0000073

[Term]
id: CASSTIME:0000185
name: cass day 112
synonym: "day112" EXACT
def: "" []
is_a: CASSTIME:0000073

[Term]
id: CASSTIME:0000186
name: cass day 113
synonym: "day113" EXACT
def: "" []
is_a: CASSTIME:0000073

[Term]
id: CASSTIME:0000187
name: cass day 114
synonym: "day114" EXACT
def: "" []
is_a: CASSTIME:0000073

[Term]
id: CASSTIME:0000188
name: cass day 115
synonym: "day115" EXACT
def: "" []
is_a: CASSTIME:0000073

[Term]
id: CASSTIME:0000189
name: cass day 116
synonym: "day116" EXACT
def: "" []
is_a: CASSTIME:0000073

[Term]
id: CASSTIME:0000190
name: cass day 117
synonym: "day117" EXACT
def: "" []
is_a: CASSTIME:0000073

[Term]
id: CASSTIME:0000191
name: cass day 118
synonym: "day118" EXACT
def: "" []
is_a: CASSTIME:0000073

[Term]
id: CASSTIME:0000192
name: cass day 119
synonym: "day119" EXACT
def: "" []
is_a: CASSTIME:0000073

[Term]
id: CASSTIME:0000193
name: cass day 120
synonym: "day120" EXACT
def: "" []
is_a: CASSTIME:0000073

[Term]
id: CASSTIME:0000194
name: cass day 121
synonym: "day121" EXACT
def: "" []
is_a: CASSTIME:0000073

[Term]
id: CASSTIME:0000195
name: cass day 122
synonym: "day122" EXACT
def: "" []
is_a: CASSTIME:0000073

[Term]
id: CASSTIME:0000196
name: cass day 123
synonym: "day123" EXACT
def: "" []
is_a: CASSTIME:0000073

[Term]
id: CASSTIME:0000197
name: cass day 124
synonym: "day124" EXACT
def: "" []
is_a: CASSTIME:0000073

[Term]
id: CASSTIME:0000198
name: cass day 125
synonym: "day125" EXACT
def: "" []
is_a: CASSTIME:0000073

[Term]
id: CASSTIME:0000199
name: cass day 126
synonym: "day126" EXACT
def: "" []
is_a: CASSTIME:0000073

[Term]
id: CASSTIME:0000200
name: cass day 127
synonym: "day127" EXACT
def: "" []
is_a: CASSTIME:0000073

[Term]
id: CASSTIME:0000201
name: cass day 128
synonym: "day128" EXACT
def: "" []
is_a: CASSTIME:0000073

[Term]
id: CASSTIME:0000202
name: cass day 129
synonym: "day129" EXACT
def: "" []
is_a: CASSTIME:0000073

[Term]
id: CASSTIME:0000203
name: cass day 130
synonym: "day130" EXACT
def: "" []
is_a: CASSTIME:0000073

[Term]
id: CASSTIME:0000204
name: cass day 131
synonym: "day131" EXACT
def: "" []
is_a: CASSTIME:0000073

[Term]
id: CASSTIME:0000205
name: cass day 132
synonym: "day132" EXACT
def: "" []
is_a: CASSTIME:0000073

[Term]
id: CASSTIME:0000206
name: cass day 133
synonym: "day133" EXACT
def: "" []
is_a: CASSTIME:0000073

[Term]
id: CASSTIME:0000207
name: cass day 134
synonym: "day134" EXACT
def: "" []
is_a: CASSTIME:0000073

[Term]
id: CASSTIME:0000208
name: cass day 135
synonym: "day135" EXACT
def: "" []
is_a: CASSTIME:0000073

[Term]
id: CASSTIME:0000209
name: cass day 136
synonym: "day136" EXACT
def: "" []
is_a: CASSTIME:0000073

[Term]
id: CASSTIME:0000210
name: cass day 137
synonym: "day137" EXACT
def: "" []
is_a: CASSTIME:0000073

[Term]
id: CASSTIME:0000211
name: cass day 138
synonym: "day138" EXACT
def: "" []
is_a: CASSTIME:0000073

[Term]
id: CASSTIME:0000212
name: cass day 139
synonym: "day139" EXACT
def: "" []
is_a: CASSTIME:0000073

[Term]
id: CASSTIME:0000213
name: cass day 140
synonym: "day140" EXACT
def: "" []
is_a: CASSTIME:0000073

[Term]
id: CASSTIME:0000214
name: cass day 141
synonym: "day141" EXACT
def: "" []
is_a: CASSTIME:0000073

[Term]
id: CASSTIME:0000215
name: cass day 142
synonym: "day142" EXACT
def: "" []
is_a: CASSTIME:0000073

[Term]
id: CASSTIME:0000216
name: cass day 143
synonym: "day143" EXACT
def: "" []
is_a: CASSTIME:0000073

[Term]
id: CASSTIME:0000217
name: cass day 144
synonym: "day144" EXACT
def: "" []
is_a: CASSTIME:0000073

[Term]
id: CASSTIME:0000218
name: cass day 145
synonym: "day145" EXACT
def: "" []
is_a: CASSTIME:0000073

[Term]
id: CASSTIME:0000219
name: cass day 146
synonym: "day146" EXACT
def: "" []
is_a: CASSTIME:0000073

[Term]
id: CASSTIME:0000220
name: cass day 147
synonym: "day147" EXACT
def: "" []
is_a: CASSTIME:0000073

[Term]
id: CASSTIME:0000221
name: cass day 148
synonym: "day148" EXACT
def: "" []
is_a: CASSTIME:0000073

[Term]
id: CASSTIME:0000222
name: cass day 149
synonym: "day149" EXACT
def: "" []
is_a: CASSTIME:0000073

[Term]
id: CASSTIME:0000223
name: cass day 150
synonym: "day150" EXACT
def: "" []
is_a: CASSTIME:0000073

[Term]
id: CASSTIME:0000224
name: cass day 151
synonym: "day151" EXACT
def: "" []
is_a: CASSTIME:0000073

[Term]
id: CASSTIME:0000225
name: cass day 152
synonym: "day152" EXACT
def: "" []
is_a: CASSTIME:0000073

[Term]
id: CASSTIME:0000226
name: cass day 153
synonym: "day153" EXACT
def: "" []
is_a: CASSTIME:0000073

[Term]
id: CASSTIME:0000227
name: cass day 154
synonym: "day154" EXACT
def: "" []
is_a: CASSTIME:0000073

[Term]
id: CASSTIME:0000228
name: cass day 155
synonym: "day155" EXACT
def: "" []
is_a: CASSTIME:0000073

[Term]
id: CASSTIME:0000229
name: cass day 156
synonym: "day156" EXACT
def: "" []
is_a: CASSTIME:0000073

[Term]
id: CASSTIME:0000230
name: cass day 157
synonym: "day157" EXACT
def: "" []
is_a: CASSTIME:0000073

[Term]
id: CASSTIME:0000231
name: cass day 158
synonym: "day158" EXACT
def: "" []
is_a: CASSTIME:0000073

[Term]
id: CASSTIME:0000232
name: cass day 159
synonym: "day159" EXACT
def: "" []
is_a: CASSTIME:0000073

[Term]
id: CASSTIME:0000233
name: cass day 160
synonym: "day160" EXACT
def: "" []
is_a: CASSTIME:0000073

[Term]
id: CASSTIME:0000234
name: cass day 161
synonym: "day161" EXACT
def: "" []
is_a: CASSTIME:0000073

[Term]
id: CASSTIME:0000235
name: cass day 162
synonym: "day162" EXACT
def: "" []
is_a: CASSTIME:0000073

[Term]
id: CASSTIME:0000236
name: cass day 163
synonym: "day163" EXACT
def: "" []
is_a: CASSTIME:0000073

[Term]
id: CASSTIME:0000237
name: cass day 164
synonym: "day164" EXACT
def: "" []
is_a: CASSTIME:0000073

[Term]
id: CASSTIME:0000238
name: cass day 165
synonym: "day165" EXACT
def: "" []
is_a: CASSTIME:0000073

[Term]
id: CASSTIME:0000239
name: cass day 166
synonym: "day166" EXACT
def: "" []
is_a: CASSTIME:0000073

[Term]
id: CASSTIME:0000240
name: cass day 167
synonym: "day167" EXACT
def: "" []
is_a: CASSTIME:0000073

[Term]
id: CASSTIME:0000241
name: cass day 168
synonym: "day168" EXACT
def: "" []
is_a: CASSTIME:0000073

[Term]
id: CASSTIME:0000242
name: cass day 169
synonym: "day169" EXACT
def: "" []
is_a: CASSTIME:0000073

[Term]
id: CASSTIME:0000243
name: cass day 170
synonym: "day170" EXACT
def: "" []
is_a: CASSTIME:0000073

[Term]
id: CASSTIME:0000244
name: cass day 171
synonym: "day171" EXACT
def: "" []
is_a: CASSTIME:0000073

[Term]
id: CASSTIME:0000245
name: cass day 172
synonym: "day172" EXACT
def: "" []
is_a: CASSTIME:0000073

[Term]
id: CASSTIME:0000246
name: cass day 173
synonym: "day173" EXACT
def: "" []
is_a: CASSTIME:0000073

[Term]
id: CASSTIME:0000247
name: cass day 174
synonym: "day174" EXACT
def: "" []
is_a: CASSTIME:0000073

[Term]
id: CASSTIME:0000248
name: cass day 175
synonym: "day175" EXACT
def: "" []
is_a: CASSTIME:0000073

[Term]
id: CASSTIME:0000249
name: cass day 176
synonym: "day176" EXACT
def: "" []
is_a: CASSTIME:0000073

[Term]
id: CASSTIME:0000250
name: cass day 177
synonym: "day177" EXACT
def: "" []
is_a: CASSTIME:0000073

[Term]
id: CASSTIME:0000251
name: cass day 178
synonym: "day178" EXACT
def: "" []
is_a: CASSTIME:0000073

[Term]
id: CASSTIME:0000252
name: cass day 179
synonym: "day179" EXACT
def: "" []
is_a: CASSTIME:0000073

[Term]
id: CASSTIME:0000253
name: cass day 180
synonym: "day180" EXACT
def: "" []
is_a: CASSTIME:0000073

[Term]
id: CASSTIME:0000254
name: cass day 181
synonym: "day181" EXACT
def: "" []
is_a: CASSTIME:0000073

[Term]
id: CASSTIME:0000255
name: cass day 182
synonym: "day182" EXACT
def: "" []
is_a: CASSTIME:0000073

[Term]
id: CASSTIME:0000256
name: cass day 183
synonym: "day183" EXACT
def: "" []
is_a: CASSTIME:0000073

[Term]
id: CASSTIME:0000257
name: cass day 184
synonym: "day184" EXACT
def: "" []
is_a: CASSTIME:0000073

[Term]
id: CASSTIME:0000258
name: cass day 185
synonym: "day185" EXACT
def: "" []
is_a: CASSTIME:0000073

[Term]
id: CASSTIME:0000259
name: cass day 186
synonym: "day186" EXACT
def: "" []
is_a: CASSTIME:0000073

[Term]
id: CASSTIME:0000260
name: cass day 187
synonym: "day187" EXACT
def: "" []
is_a: CASSTIME:0000073

[Term]
id: CASSTIME:0000261
name: cass day 188
synonym: "day188" EXACT
def: "" []
is_a: CASSTIME:0000073

[Term]
id: CASSTIME:0000262
name: cass day 189
synonym: "day189" EXACT
def: "" []
is_a: CASSTIME:0000073

[Term]
id: CASSTIME:0000263
name: cass day 190
synonym: "day190" EXACT
def: "" []
is_a: CASSTIME:0000073

[Term]
id: CASSTIME:0000264
name: cass day 191
synonym: "day191" EXACT
def: "" []
is_a: CASSTIME:0000073

[Term]
id: CASSTIME:0000265
name: cass day 192
synonym: "day192" EXACT
def: "" []
is_a: CASSTIME:0000073

[Term]
id: CASSTIME:0000266
name: cass day 193
synonym: "day193" EXACT
def: "" []
is_a: CASSTIME:0000073

[Term]
id: CASSTIME:0000267
name: cass day 194
synonym: "day194" EXACT
def: "" []
is_a: CASSTIME:0000073

[Term]
id: CASSTIME:0000268
name: cass day 195
synonym: "day195" EXACT
def: "" []
is_a: CASSTIME:0000073

[Term]
id: CASSTIME:0000269
name: cass day 196
synonym: "day196" EXACT
def: "" []
is_a: CASSTIME:0000073

[Term]
id: CASSTIME:0000270
name: cass day 197
synonym: "day197" EXACT
def: "" []
is_a: CASSTIME:0000073

[Term]
id: CASSTIME:0000271
name: cass day 198
synonym: "day198" EXACT
def: "" []
is_a: CASSTIME:0000073

[Term]
id: CASSTIME:0000272
name: cass day 199
synonym: "day199" EXACT
def: "" []
is_a: CASSTIME:0000073

[Term]
id: CASSTIME:0000273
name: cass day 200
synonym: "day200" EXACT
def: "" []
is_a: CASSTIME:0000073

[Term]
id: CASSTIME:0000274
name: cass day 201
synonym: "day201" EXACT
def: "" []
is_a: CASSTIME:0000073

[Term]
id: CASSTIME:0000275
name: cass day 202
synonym: "day202" EXACT
def: "" []
is_a: CASSTIME:0000073

[Term]
id: CASSTIME:0000276
name: cass day 203
synonym: "day203" EXACT
def: "" []
is_a: CASSTIME:0000073

[Term]
id: CASSTIME:0000277
name: cass day 204
synonym: "day204" EXACT
def: "" []
is_a: CASSTIME:0000073

[Term]
id: CASSTIME:0000278
name: cass day 205
synonym: "day205" EXACT
def: "" []
is_a: CASSTIME:0000073

[Term]
id: CASSTIME:0000279
name: cass day 206
synonym: "day206" EXACT
def: "" []
is_a: CASSTIME:0000073

[Term]
id: CASSTIME:0000280
name: cass day 207
synonym: "day207" EXACT
def: "" []
is_a: CASSTIME:0000073

[Term]
id: CASSTIME:0000281
name: cass day 208
synonym: "day208" EXACT
def: "" []
is_a: CASSTIME:0000073

[Term]
id: CASSTIME:0000282
name: cass day 209
synonym: "day209" EXACT
def: "" []
is_a: CASSTIME:0000073

[Term]
id: CASSTIME:0000283
name: cass day 210
synonym: "day210" EXACT
def: "" []
is_a: CASSTIME:0000073

[Term]
id: CASSTIME:0000284
name: cass day 211
synonym: "day211" EXACT
def: "" []
is_a: CASSTIME:0000073

[Term]
id: CASSTIME:0000285
name: cass day 212
synonym: "day212" EXACT
def: "" []
is_a: CASSTIME:0000073

[Term]
id: CASSTIME:0000286
name: cass day 213
synonym: "day213" EXACT
def: "" []
is_a: CASSTIME:0000073

[Term]
id: CASSTIME:0000287
name: cass day 214
synonym: "day214" EXACT
def: "" []
is_a: CASSTIME:0000073

[Term]
id: CASSTIME:0000288
name: cass day 215
synonym: "day215" EXACT
def: "" []
is_a: CASSTIME:0000073

[Term]
id: CASSTIME:0000289
name: cass day 216
synonym: "day216" EXACT
def: "" []
is_a: CASSTIME:0000073

[Term]
id: CASSTIME:0000290
name: cass day 217
synonym: "day217" EXACT
def: "" []
is_a: CASSTIME:0000073

[Term]
id: CASSTIME:0000291
name: cass day 218
synonym: "day218" EXACT
def: "" []
is_a: CASSTIME:0000073

[Term]
id: CASSTIME:0000292
name: cass day 219
synonym: "day219" EXACT
def: "" []
is_a: CASSTIME:0000073

[Term]
id: CASSTIME:0000293
name: cass day 220
synonym: "day220" EXACT
def: "" []
is_a: CASSTIME:0000073

[Term]
id: CASSTIME:0000294
name: cass day 221
synonym: "day221" EXACT
def: "" []
is_a: CASSTIME:0000073

[Term]
id: CASSTIME:0000295
name: cass day 222
synonym: "day222" EXACT
def: "" []
is_a: CASSTIME:0000073

[Term]
id: CASSTIME:0000296
name: cass day 223
synonym: "day223" EXACT
def: "" []
is_a: CASSTIME:0000073

[Term]
id: CASSTIME:0000297
name: cass day 224
synonym: "day224" EXACT
def: "" []
is_a: CASSTIME:0000073

[Term]
id: CASSTIME:0000298
name: cass day 225
synonym: "day225" EXACT
def: "" []
is_a: CASSTIME:0000073

[Term]
id: CASSTIME:0000299
name: cass day 226
synonym: "day226" EXACT
def: "" []
is_a: CASSTIME:0000073

[Term]
id: CASSTIME:0000300
name: cass day 227
synonym: "day227" EXACT
def: "" []
is_a: CASSTIME:0000073

[Term]
id: CASSTIME:0000301
name: cass day 228
synonym: "day228" EXACT
def: "" []
is_a: CASSTIME:0000073

[Term]
id: CASSTIME:0000302
name: cass day 229
synonym: "day229" EXACT
def: "" []
is_a: CASSTIME:0000073

[Term]
id: CASSTIME:0000303
name: cass day 230
synonym: "day230" EXACT
def: "" []
is_a: CASSTIME:0000073

[Term]
id: CASSTIME:0000304
name: cass day 231
synonym: "day231" EXACT
def: "" []
is_a: CASSTIME:0000073

[Term]
id: CASSTIME:0000305
name: cass day 232
synonym: "day232" EXACT
def: "" []
is_a: CASSTIME:0000073

[Term]
id: CASSTIME:0000306
name: cass day 233
synonym: "day233" EXACT
def: "" []
is_a: CASSTIME:0000073

[Term]
id: CASSTIME:0000307
name: cass day 234
synonym: "day234" EXACT
def: "" []
is_a: CASSTIME:0000073

[Term]
id: CASSTIME:0000308
name: cass day 235
synonym: "day235" EXACT
def: "" []
is_a: CASSTIME:0000073

[Term]
id: CASSTIME:0000309
name: cass day 236
synonym: "day236" EXACT
def: "" []
is_a: CASSTIME:0000073

[Term]
id: CASSTIME:0000310
name: cass day 237
synonym: "day237" EXACT
def: "" []
is_a: CASSTIME:0000073

[Term]
id: CASSTIME:0000311
name: cass day 238
synonym: "day238" EXACT
def: "" []
is_a: CASSTIME:0000073

[Term]
id: CASSTIME:0000312
name: cass day 239
synonym: "day239" EXACT
def: "" []
is_a: CASSTIME:0000073

[Term]
id: CASSTIME:0000313
name: cass day 240
synonym: "day240" EXACT
def: "" []
is_a: CASSTIME:0000073

[Term]
id: CASSTIME:0000314
name: cass day 241
synonym: "day241" EXACT
def: "" []
is_a: CASSTIME:0000073

[Term]
id: CASSTIME:0000315
name: cass day 242
synonym: "day242" EXACT
def: "" []
is_a: CASSTIME:0000073

[Term]
id: CASSTIME:0000316
name: cass day 243
synonym: "day243" EXACT
def: "" []
is_a: CASSTIME:0000073

[Term]
id: CASSTIME:0000317
name: cass day 244
synonym: "day244" EXACT
def: "" []
is_a: CASSTIME:0000073

[Term]
id: CASSTIME:0000318
name: cass day 245
synonym: "day245" EXACT
def: "" []
is_a: CASSTIME:0000073

[Term]
id: CASSTIME:0000319
name: cass day 246
synonym: "day246" EXACT
def: "" []
is_a: CASSTIME:0000073

[Term]
id: CASSTIME:0000320
name: cass day 247
synonym: "day247" EXACT
def: "" []
is_a: CASSTIME:0000073

[Term]
id: CASSTIME:0000321
name: cass day 248
synonym: "day248" EXACT
def: "" []
is_a: CASSTIME:0000073

[Term]
id: CASSTIME:0000322
name: cass day 249
synonym: "day249" EXACT
def: "" []
is_a: CASSTIME:0000073

[Term]
id: CASSTIME:0000323
name: cass day 250
synonym: "day250" EXACT
def: "" []
is_a: CASSTIME:0000073

[Term]
id: CASSTIME:0000324
name: cass day 251
synonym: "day251" EXACT
def: "" []
is_a: CASSTIME:0000073

[Term]
id: CASSTIME:0000325
name: cass day 252
synonym: "day252" EXACT
def: "" []
is_a: CASSTIME:0000073

[Term]
id: CASSTIME:0000326
name: cass day 253
synonym: "day253" EXACT
def: "" []
is_a: CASSTIME:0000073

[Term]
id: CASSTIME:0000327
name: cass day 254
synonym: "day254" EXACT
def: "" []
is_a: CASSTIME:0000073

[Term]
id: CASSTIME:0000328
name: cass day 255
synonym: "day255" EXACT
def: "" []
is_a: CASSTIME:0000073

[Term]
id: CASSTIME:0000329
name: cass day 256
synonym: "day256" EXACT
def: "" []
is_a: CASSTIME:0000073

[Term]
id: CASSTIME:0000330
name: cass day 257
synonym: "day257" EXACT
def: "" []
is_a: CASSTIME:0000073

[Term]
id: CASSTIME:0000331
name: cass day 258
synonym: "day258" EXACT
def: "" []
is_a: CASSTIME:0000073

[Term]
id: CASSTIME:0000332
name: cass day 259
synonym: "day259" EXACT
def: "" []
is_a: CASSTIME:0000073

[Term]
id: CASSTIME:0000333
name: cass day 260
synonym: "day260" EXACT
def: "" []
is_a: CASSTIME:0000073

[Term]
id: CASSTIME:0000334
name: cass day 261
synonym: "day261" EXACT
def: "" []
is_a: CASSTIME:0000073

[Term]
id: CASSTIME:0000335
name: cass day 262
synonym: "day262" EXACT
def: "" []
is_a: CASSTIME:0000073

[Term]
id: CASSTIME:0000336
name: cass day 263
synonym: "day263" EXACT
def: "" []
is_a: CASSTIME:0000073

[Term]
id: CASSTIME:0000337
name: cass day 264
synonym: "day264" EXACT
def: "" []
is_a: CASSTIME:0000073

[Term]
id: CASSTIME:0000338
name: cass day 265
synonym: "day265" EXACT
def: "" []
is_a: CASSTIME:0000073

[Term]
id: CASSTIME:0000339
name: cass day 266
synonym: "day266" EXACT
def: "" []
is_a: CASSTIME:0000073

[Term]
id: CASSTIME:0000340
name: cass day 267
synonym: "day267" EXACT
def: "" []
is_a: CASSTIME:0000073

[Term]
id: CASSTIME:0000341
name: cass day 268
synonym: "day268" EXACT
def: "" []
is_a: CASSTIME:0000073

[Term]
id: CASSTIME:0000342
name: cass day 269
synonym: "day269" EXACT
def: "" []
is_a: CASSTIME:0000073

[Term]
id: CASSTIME:0000343
name: cass day 270
synonym: "day270" EXACT
def: "" []
is_a: CASSTIME:0000073

[Term]
id: CASSTIME:0000344
name: cass day 271
synonym: "day271" EXACT
def: "" []
is_a: CASSTIME:0000073

[Term]
id: CASSTIME:0000345
name: cass day 272
synonym: "day272" EXACT
def: "" []
is_a: CASSTIME:0000073

[Term]
id: CASSTIME:0000346
name: cass day 273
synonym: "day273" EXACT
def: "" []
is_a: CASSTIME:0000073

[Term]
id: CASSTIME:0000347
name: cass day 274
synonym: "day274" EXACT
def: "" []
is_a: CASSTIME:0000073

[Term]
id: CASSTIME:0000348
name: cass day 275
synonym: "day275" EXACT
def: "" []
is_a: CASSTIME:0000073

[Term]
id: CASSTIME:0000349
name: cass day 276
synonym: "day276" EXACT
def: "" []
is_a: CASSTIME:0000073

[Term]
id: CASSTIME:0000350
name: cass day 277
synonym: "day277" EXACT
def: "" []
is_a: CASSTIME:0000073

[Term]
id: CASSTIME:0000351
name: cass day 278
synonym: "day278" EXACT
def: "" []
is_a: CASSTIME:0000073

[Term]
id: CASSTIME:0000352
name: cass day 279
synonym: "day279" EXACT
def: "" []
is_a: CASSTIME:0000073

[Term]
id: CASSTIME:0000353
name: cass day 280
synonym: "day280" EXACT
def: "" []
is_a: CASSTIME:0000073

[Term]
id: CASSTIME:0000354
name: cass day 281
synonym: "day281" EXACT
def: "" []
is_a: CASSTIME:0000073

[Term]
id: CASSTIME:0000355
name: cass day 282
synonym: "day282" EXACT
def: "" []
is_a: CASSTIME:0000073

[Term]
id: CASSTIME:0000356
name: cass day 283
synonym: "day283" EXACT
def: "" []
is_a: CASSTIME:0000073

[Term]
id: CASSTIME:0000357
name: cass day 284
synonym: "day284" EXACT
def: "" []
is_a: CASSTIME:0000073

[Term]
id: CASSTIME:0000358
name: cass day 285
synonym: "day285" EXACT
def: "" []
is_a: CASSTIME:0000073

[Term]
id: CASSTIME:0000359
name: cass day 286
synonym: "day286" EXACT
def: "" []
is_a: CASSTIME:0000073

[Term]
id: CASSTIME:0000360
name: cass day 287
synonym: "day287" EXACT
def: "" []
is_a: CASSTIME:0000073

[Term]
id: CASSTIME:0000361
name: cass day 288
synonym: "day288" EXACT
def: "" []
is_a: CASSTIME:0000073

[Term]
id: CASSTIME:0000362
name: cass day 289
synonym: "day289" EXACT
def: "" []
is_a: CASSTIME:0000073

[Term]
id: CASSTIME:0000363
name: cass day 290
synonym: "day290" EXACT
def: "" []
is_a: CASSTIME:0000073

[Term]
id: CASSTIME:0000364
name: cass day 291
synonym: "day291" EXACT
def: "" []
is_a: CASSTIME:0000073

[Term]
id: CASSTIME:0000365
name: cass day 292
synonym: "day292" EXACT
def: "" []
is_a: CASSTIME:0000073

[Term]
id: CASSTIME:0000366
name: cass day 293
synonym: "day293" EXACT
def: "" []
is_a: CASSTIME:0000073

[Term]
id: CASSTIME:0000367
name: cass day 294
synonym: "day294" EXACT
def: "" []
is_a: CASSTIME:0000073

[Term]
id: CASSTIME:0000368
name: cass day 295
synonym: "day295" EXACT
def: "" []
is_a: CASSTIME:0000073

[Term]
id: CASSTIME:0000369
name: cass day 296
synonym: "day296" EXACT
def: "" []
is_a: CASSTIME:0000073

[Term]
id: CASSTIME:0000370
name: cass day 297
synonym: "day297" EXACT
def: "" []
is_a: CASSTIME:0000073

[Term]
id: CASSTIME:0000371
name: cass day 298
synonym: "day298" EXACT
def: "" []
is_a: CASSTIME:0000073

[Term]
id: CASSTIME:0000372
name: cass day 299
synonym: "day299" EXACT
def: "" []
is_a: CASSTIME:0000073

[Term]
id: CASSTIME:0000373
name: cass day 300
synonym: "day300" EXACT
def: "" []
is_a: CASSTIME:0000073

[Term]
id: CASSTIME:0000374
name: cass day 301
synonym: "day301" EXACT
def: "" []
is_a: CASSTIME:0000073

[Term]
id: CASSTIME:0000375
name: cass day 302
synonym: "day302" EXACT
def: "" []
is_a: CASSTIME:0000073

[Term]
id: CASSTIME:0000376
name: cass day 303
synonym: "day303" EXACT
def: "" []
is_a: CASSTIME:0000073

[Term]
id: CASSTIME:0000377
name: cass day 304
synonym: "day304" EXACT
def: "" []
is_a: CASSTIME:0000073

[Term]
id: CASSTIME:0000378
name: cass day 305
synonym: "day305" EXACT
def: "" []
is_a: CASSTIME:0000073

[Term]
id: CASSTIME:0000379
name: cass day 306
synonym: "day306" EXACT
def: "" []
is_a: CASSTIME:0000073

[Term]
id: CASSTIME:0000380
name: cass day 307
synonym: "day307" EXACT
def: "" []
is_a: CASSTIME:0000073

[Term]
id: CASSTIME:0000381
name: cass day 308
synonym: "day308" EXACT
def: "" []
is_a: CASSTIME:0000073

[Term]
id: CASSTIME:0000382
name: cass day 309
synonym: "day309" EXACT
def: "" []
is_a: CASSTIME:0000073

[Term]
id: CASSTIME:0000383
name: cass day 310
synonym: "day310" EXACT
def: "" []
is_a: CASSTIME:0000073

[Term]
id: CASSTIME:0000384
name: cass day 311
synonym: "day311" EXACT
def: "" []
is_a: CASSTIME:0000073

[Term]
id: CASSTIME:0000385
name: cass day 312
synonym: "day312" EXACT
def: "" []
is_a: CASSTIME:0000073

[Term]
id: CASSTIME:0000386
name: cass day 313
synonym: "day313" EXACT
def: "" []
is_a: CASSTIME:0000073

[Term]
id: CASSTIME:0000387
name: cass day 314
synonym: "day314" EXACT
def: "" []
is_a: CASSTIME:0000073

[Term]
id: CASSTIME:0000388
name: cass day 315
synonym: "day315" EXACT
def: "" []
is_a: CASSTIME:0000073

[Term]
id: CASSTIME:0000389
name: cass day 316
synonym: "day316" EXACT
def: "" []
is_a: CASSTIME:0000073

[Term]
id: CASSTIME:0000390
name: cass day 317
synonym: "day317" EXACT
def: "" []
is_a: CASSTIME:0000073

[Term]
id: CASSTIME:0000391
name: cass day 318
synonym: "day318" EXACT
def: "" []
is_a: CASSTIME:0000073

[Term]
id: CASSTIME:0000392
name: cass day 319
synonym: "day319" EXACT
def: "" []
is_a: CASSTIME:0000073

[Term]
id: CASSTIME:0000393
name: cass day 320
synonym: "day320" EXACT
def: "" []
is_a: CASSTIME:0000073

[Term]
id: CASSTIME:0000394
name: cass day 321
synonym: "day321" EXACT
def: "" []
is_a: CASSTIME:0000073

[Term]
id: CASSTIME:0000395
name: cass day 322
synonym: "day322" EXACT
def: "" []
is_a: CASSTIME:0000073

[Term]
id: CASSTIME:0000396
name: cass day 323
synonym: "day323" EXACT
def: "" []
is_a: CASSTIME:0000073

[Term]
id: CASSTIME:0000397
name: cass day 324
synonym: "day324" EXACT
def: "" []
is_a: CASSTIME:0000073

[Term]
id: CASSTIME:0000398
name: cass day 325
synonym: "day325" EXACT
def: "" []
is_a: CASSTIME:0000073

[Term]
id: CASSTIME:0000399
name: cass day 326
synonym: "day326" EXACT
def: "" []
is_a: CASSTIME:0000073

[Term]
id: CASSTIME:0000400
name: cass day 327
synonym: "day327" EXACT
def: "" []
is_a: CASSTIME:0000073

[Term]
id: CASSTIME:0000401
name: cass day 328
synonym: "day328" EXACT
def: "" []
is_a: CASSTIME:0000073

[Term]
id: CASSTIME:0000402
name: cass day 329
synonym: "day329" EXACT
def: "" []
is_a: CASSTIME:0000073

[Term]
id: CASSTIME:0000403
name: cass day 330
synonym: "day330" EXACT
def: "" []
is_a: CASSTIME:0000073

[Term]
id: CASSTIME:0000404
name: cass day 331
synonym: "day331" EXACT
def: "" []
is_a: CASSTIME:0000073

[Term]
id: CASSTIME:0000405
name: cass day 332
synonym: "day332" EXACT
def: "" []
is_a: CASSTIME:0000073

[Term]
id: CASSTIME:0000406
name: cass day 333
synonym: "day333" EXACT
def: "" []
is_a: CASSTIME:0000073

[Term]
id: CASSTIME:0000407
name: cass day 334
synonym: "day334" EXACT
def: "" []
is_a: CASSTIME:0000073

[Term]
id: CASSTIME:0000408
name: cass day 335
synonym: "day335" EXACT
def: "" []
is_a: CASSTIME:0000073

[Term]
id: CASSTIME:0000409
name: cass day 336
synonym: "day336" EXACT
def: "" []
is_a: CASSTIME:0000073

[Term]
id: CASSTIME:0000410
name: cass day 337
synonym: "day337" EXACT
def: "" []
is_a: CASSTIME:0000073

[Term]
id: CASSTIME:0000411
name: cass day 338
synonym: "day338" EXACT
def: "" []
is_a: CASSTIME:0000073

[Term]
id: CASSTIME:0000412
name: cass day 339
synonym: "day339" EXACT
def: "" []
is_a: CASSTIME:0000073

[Term]
id: CASSTIME:0000413
name: cass day 340
synonym: "day340" EXACT
def: "" []
is_a: CASSTIME:0000073

[Term]
id: CASSTIME:0000414
name: cass day 341
synonym: "day341" EXACT
def: "" []
is_a: CASSTIME:0000073

[Term]
id: CASSTIME:0000415
name: cass day 342
synonym: "day342" EXACT
def: "" []
is_a: CASSTIME:0000073

[Term]
id: CASSTIME:0000416
name: cass day 343
synonym: "day343" EXACT
def: "" []
is_a: CASSTIME:0000073

[Term]
id: CASSTIME:0000417
name: cass day 344
synonym: "day344" EXACT
def: "" []
is_a: CASSTIME:0000073

[Term]
id: CASSTIME:0000418
name: cass day 345
synonym: "day345" EXACT
def: "" []
is_a: CASSTIME:0000073

[Term]
id: CASSTIME:0000419
name: cass day 346
synonym: "day346" EXACT
def: "" []
is_a: CASSTIME:0000073

[Term]
id: CASSTIME:0000420
name: cass day 347
synonym: "day347" EXACT
def: "" []
is_a: CASSTIME:0000073

[Term]
id: CASSTIME:0000421
name: cass day 348
synonym: "day348" EXACT
def: "" []
is_a: CASSTIME:0000073

[Term]
id: CASSTIME:0000422
name: cass day 349
synonym: "day349" EXACT
def: "" []
is_a: CASSTIME:0000073

[Term]
id: CASSTIME:0000423
name: cass day 350
synonym: "day350" EXACT
def: "" []
is_a: CASSTIME:0000073

[Term]
id: CASSTIME:0000424
name: cass day 351
synonym: "day351" EXACT
def: "" []
is_a: CASSTIME:0000073

[Term]
id: CASSTIME:0000425
name: cass day 352
synonym: "day352" EXACT
def: "" []
is_a: CASSTIME:0000073

[Term]
id: CASSTIME:0000426
name: cass day 353
synonym: "day353" EXACT
def: "" []
is_a: CASSTIME:0000073

[Term]
id: CASSTIME:0000427
name: cass day 354
synonym: "day354" EXACT
def: "" []
is_a: CASSTIME:0000073

[Term]
id: CASSTIME:0000428
name: cass day 355
synonym: "day355" EXACT
def: "" []
is_a: CASSTIME:0000073

[Term]
id: CASSTIME:0000429
name: cass day 356
synonym: "day356" EXACT
def: "" []
is_a: CASSTIME:0000073

[Term]
id: CASSTIME:0000430
name: cass day 357
synonym: "day357" EXACT
def: "" []
is_a: CASSTIME:0000073

[Term]
id: CASSTIME:0000431
name: cass day 358
synonym: "day358" EXACT
def: "" []
is_a: CASSTIME:0000073

[Term]
id: CASSTIME:0000432
name: cass day 359
synonym: "day359" EXACT
def: "" []
is_a: CASSTIME:0000073

[Term]
id: CASSTIME:0000433
name: cass day 360
synonym: "day360" EXACT
def: "" []
is_a: CASSTIME:0000073

[Term]
id: CASSTIME:0000434
name: cass day 361
synonym: "day361" EXACT
def: "" []
is_a: CASSTIME:0000073

[Term]
id: CASSTIME:0000435
name: cass day 362
synonym: "day362" EXACT
def: "" []
is_a: CASSTIME:0000073

[Term]
id: CASSTIME:0000436
name: cass day 363
synonym: "day363" EXACT
def: "" []
is_a: CASSTIME:0000073

[Term]
id: CASSTIME:0000437
name: cass day 364
synonym: "day364" EXACT
def: "" []
is_a: CASSTIME:0000073

[Term]
id: CASSTIME:0000438
name: cass day 365
synonym: "day365" EXACT
def: "" []
is_a: CASSTIME:0000073
